%Text Books : \cite{apostol}, \cite{rudin}
%Module 1:
%The Weirstrass theorem, other forms of Fourier series, the Fourier integral theorem, the exponential form of the Fourier integral theorem, integral transforms and convolutions, the convolution theorem for Fourier transforms.
%(Chapter 11 Sections 11.15 to 11.21 of \cite{apostol}) (20 hours.)
%Module 2:
%Multivariable Differential Calculus, The directional derivative, directional derivatives and continuity, the total derivative, the total derivative expressed in terms of partial derivatives, An application of complex- valued functions, the matrix of a linear function, the Jacobian matrix, the matrix form of the chain rule. Implicit functions and extremum problems, the mean value theorem for differentiable functions,
%(Chapter 12 Sections. 12.1 to 12.11 of \cite{apostol}) (22 hours.)
%Module 3: 
%A sufficient condition for differentiability, a sufficient condition for equality of mixed partial derivatives, functions with non-zero Jacobian determinant, the inverse function theorem ,the implicit function theorem, extrema of real- valued functions of one variable, extrema of real-valued functions of several variables.
%Chapter 12 Sections-. 12.12 to 12.13 of \cite{apostol} 
%Chapter 13 Sections-. 13.1 to 13.6 of \cite{apostol} (28 hours.)
%Module 4:
%Integration of Differential Forms Integration, primitive mappings, partitions of unity, change of variables, differential forms.
%(Chapter 10 Sections. 10.1 to 10.14 of \cite{rudin}) (20 hours)

\part{ME010303 Multivariate Calculus \& Integral Transforms}
%Module 1 - \cite{apostol} 11
%Module 2 - \cite{apostol} 12
%Module 3 - \cite{apostol} 12, 13
%Module 4 - \cite{rudin} 10
%\cite{apostol}
%\chapter{The Real and Complex Number Systems*}
%\chapter{Some Basic Notations of Set Theory*}
%\chapter{Elements of Point Set Topology*}
%\chapter{Limits and Continuity*}
%\chapter{Derivatives*}
%\chapter{Functions of Bounded Variation and Rectifiable Curves*}
%\chapter{The Riemann-Stieltjes Integral*}
%\chapter{Infinite Series adn Infinite Products*}
%\chapter{Sequences of Functions*}
%\chapter{The Lebesgue Integral*}
\chapter{Fourier Series and Fourier Integrals}
\section{The Weierstrass Approximation Theorem}
	Every continuous, real valued function on a compact interval has a polynomial approximation.\cite[Theorem 11.17]{apostol}
	\begin{theorem}[Weierstrass]
		Let $f$ be a real-valued, continuous function on a compact interval $[a,b]$. Then for every $\epsilon > 0$, there is a polynomial $p$ such that $|f(x)-p(x)| < \epsilon$ for every $x \in [a,b]$.
	\end{theorem}
	\begin{synopsis}
		Given a real-valued continuous function on compact interval $[a,b]$, we can construct a real-valued, continous function $g$ on $\mathbb{R}$ which is periodic with period $2\pi$. We have, if $f \in L(I)$ and $f$ is bounded almost everywhere in $I$, then $f \in L^2(I)$.\cite[Theorem 10.52]{apostol}.By Fejer's theorem (\cite[Theorem 11.15]{apostol}), the fourier series generated by $g$ (\cite[definition 11.3]{apostol}) converges to the Cesaro sum (\cite[Definition 8.47]{apostol}), which is $g$ itself in this case. Thus for any $\epsilon > 0$, there is a finite sum of trignometric functions. The power series expansions of trignometric functions (\cite[definition 9.27]{apostol}) being uniformly convergent, there exists a polynomial $p_m$ which approximates $g$. And we can construct $p$ (polynomial approximation of $g$) using $p_m$.
	\end{synopsis}
	\begin{proof}
		Define $g : \mathbb{R} \to \mathbb{R}$,
		$$ g(t) = \begin{cases}
			f(a+(b-a)t/\pi),\ t \in [0,\pi) \\
			f(a+(2\pi-t)(b-a)/\pi),\ t \in [\pi,2\pi] \\
			g(t - 2n\pi),\ t > 2\pi,\ n \in \mathbb{N} \\
			g(t+2n\pi),\ t < 0,\ n \in \mathbb{N}
			\end{cases}$$

		Thus $g$ is a continuous, real-valued, periodic function with period $2\pi$ such that
		\begin{equation}
			f(x) = g\left(\frac{\pi (x-a)}{b-a}\right),\ x \in [a,b]
			\label{equ:fx}
		\end{equation}

		The fourier series generated by $g$ is given by,
		$$ g(t) \sim \frac{a_0}{2} + \sum_{k=1}^\infty \left( a_k \cos kt + b_k \sin kt \right)$$
		$$ \text{ where } a_k = \frac{1}{\pi} \int_0^{2\pi} f(t) \cos kt\ dt,\ b_k = \frac{1}{\pi} \int_0^{2\pi} f(t) \sin kt\ dt$$

		Let $\{s_n(t)\}$ be the sequence of partial sums of the fourier series generated by $g$. And $\{\sigma_n(t)\}$  be the sequence of averages of $s_n(t)$ given by,
		$$\sigma_n(t) = \frac{1}{n} \sum_{k = 1}^n s_k(t),\text{ where } s_k(t) = \frac{a_0}{2} + \sum_{j = 1}^k \left( a_j \cos jt + b_j \sin jt \right)$$

		Function $f \in L(I)$ being real-valued continuous function on a compact interval, it is bounded and hence is Lebesgue square integrable.ie, $f \in L^2(I)$. Thus, $g \in L^2(I)$.\\

		Since $g$ is continous on $\mathbb{R}$, the function $s : \mathbb{R} \to \mathbb{R}$ defined by,
		$$ s(t) = \lim_{h \to 0^+} \frac{g(t+h)-g(t-h)}{2} $$
		is well-defined on $\mathbb{R}$ and $s(t) = g(t),\ \forall t \in \mathbb{R}$.\\

		Then by Fejer's Theorem, the sequence $\{\sigma_n(t)\}$ converges uniformly to $g(t)$ for every $t \in \mathbb{R}$. Thus, given $\epsilon > 0$, there exists $N \in \mathbb{N}$ such that $\forall t \in \mathbb{R}$, $|g(t)-\sigma_N(t)| < \frac{\epsilon}{2}$.\\

		We have,
		\begin{equation}
			\sigma_N(t) = \sum_{k=0}^N \left(A_k \cos kt + B_k \sin kt \right),\text{ where } A_k, B_k \in \mathbb{R}
			\label{equ:sigmaN}
		\end{equation}
		By the power series expansion of the trignometric functions about origin,
		\begin{equation}
			\cos kt = \sum_{j = 1}^\infty \left(\frac{\cos^{(j)} 0}{j!} (kt)^j \right)  = \sum_{j = 1}^\infty A_j' t^j \text{ where } A_j' \in \mathbb{R}
			\label{equ:coskt}
		\end{equation}
		\begin{equation}
			\sin kt = \sum_{j = 1}^\infty \left(\frac{\sin^{(j)} 0}{j!} (kt)^j \right)  = \sum_{j = 1}^\infty B_j' t^j \text{ where } B_j' \in \mathbb{R}
			\label{equ:sinkt}
		\end{equation}

		Since the above power series expansions of trignometric functions are uniformly convergent, their finite linear combination $\sigma_N(t)$ is also uniformly convergent. ie, Given $\epsilon > 0$ there exists $m \in \mathbb{N}$ such that for every $t \in \mathbb{R}$
		$$\left|\sum_{k = 0}^m C_k t^k - \sigma_N(t)\right| < \frac{\epsilon}{2} \text{ where } C_k \in \mathbb{R}$$

		Therefore, $| p_m(t) - g(t)| \le | p_m(t) - \sigma_N(t) | + |\sigma_N(t) - g(t)| < \epsilon$ where $p_m(t) = \sum_{k = 0}^m C_k t^k$. Define $p : [a,b] \to \mathbb{R}$ by,
		\begin{equation}
			p(x) = p_m\left( \frac{\pi(x-a)}{b-a} \right)
			\label{equ:px}
		\end{equation}

		By equations \ref{equ:fx} and \ref{equ:px}, $|p(x)-f(x)| < \epsilon$ for every $x \in [a,b]$.
	\end{proof}
\section{Other Forms of Fourier Series}
	Let $f \in L([0,2\pi])$, then the fourier series generated by $f$ is given by,
	$$f(x) \sim \frac{a_0}{2}+\sum_{n=1}^\infty \left( a_n \cos nx + b_n \sin nx \right) $$
	$$ \text{ where } a_n = \frac{1}{\pi} \int_0^{2\pi} f(t) \cos nt\ dt,\qquad b_n = \frac{1}{\pi} \int_0^{2\pi} f(t) \sin nt\ dt$$.

	We have, $\cos nx = \frac{(e^{inx}+e^{-inx})}{2}$ and $\sin nx = \frac{(e^{inx}-e^{-inx})}{2i}$,\\
	since $e^{\pm inx} = \cos nx \pm i \sin nx$.

	$$f(x) \sim \frac{a_0}{2} + \sum_{n=1}^\infty \left( \alpha_n e^{inx} + \beta_n e^{-inx} \right)$$

	$$\text{ where } \alpha_n = \frac{(a_n - ib_n)}{2} \qquad \beta_n = \frac{(a_n+ib_n)}{2}$$

	Therefore, by assigning $\alpha_0 = a_0/2$, $\alpha_{-n} = \beta_n$, we get the following exponential form of fourier series generated by $f$,

	$$f(x) \sim \sum_{n = -\infty}^\infty \alpha_n e^{inx} \text{ where } \alpha_n = \frac{1}{2\pi} \int_0^{2\pi} f(t)\ e^{-int}\ dt$$

	Note : If $f$ is periodic with period $2\pi$, then the interval of integration $[0,2\pi]$ can be replaced with any interval of length $2\pi$. eg. $[-\pi,\pi]$

\subsection{Periodic with period $p$}
	Let $f \in L([0,p])$ and $f$ is periodic with period $p$. Then
	$$ f(x) \sim \frac{a_0}{2} + \sum_{n=1}^\infty \left( a_n \cos \frac{2\pi nx}{p} + b_n \sin \frac{2\pi nx}{p} \right) $$
	$$ \text{ where } a_n = \frac{2}{p} \int_0^p f(t) \cos \frac{2\pi nt}{p}\ dt \qquad b_n = \frac{2}{p} \int_0^p f(t) \sin \frac{2\pi nt}{p}\ dt$$
	Therefore, we have the exponential form of the above fourier series given by,
	$$ f(x) \sim \sum_{n = -\infty}^\infty \alpha_n e^\frac{2\pi inx}{p},\text{ where } \alpha_n = \frac{1}{p} \int_0^p f(t)\ e^\frac{-2\pi int}{p}\ dt$$
	
\section{Fourier Integral Theorem}

\begin{theorem}[Fourier Integral Theorem]
	Let $f \in L(-\infty,\infty)$. Suppose $x \in \mathbb{R}$ and an interval $[x-\delta,x+\delta]$ about $x$ such that either 
	\begin{enumerate}
		\item $f$ is of bounded variation on an interval $[x-\delta,x+\delta]$ about $x$ or
		\item both limits $f(x+)$ and $f(x-)$ exists and both Lebesgue intergrals
			$$\int_0^\delta \frac{f(x+t)-f(x+)}{t} dt \text{ and }\int_0^\delta \frac{f(x-t)-f(x-)}{t} dt$$
			exists.
	\end{enumerate}
	Then, 
	$$\frac{f(x+)+f(x-)}{2} = \frac{1}{\pi} \int_0^\infty \int_{-\infty}^\infty f(u)\cos v(u-x)\ du\ dv,$$
	the integral $\int_0^\infty$ being an improper Riemann integral.
\end{theorem}
\begin{synopsis}
	$$f(x+t)\frac{\sin \alpha t}{\pi t} dt \to f(u)\frac{\sin \alpha(u-x)}{\pi(u-x)} \to \frac{f(u)}{\pi} \int_0^\alpha \cos v(u-x) dv$$
	By Riemann-Lebesgue lemma\cite[Theorem 11.6]{apostol},
	$$f \in L(I) \implies \lim_{\alpha \to +\infty} \int_I f(x) \sin \alpha t\ dt = 0$$
	By Jordan's Theorem\cite[Theorem 10.8]{apostol}, if $g$ is of bounded variation on $[0,\delta]$, then
	$$\lim_{\alpha \to +\infty} \frac{2}{\pi} \int_0^\delta g(t) \frac{\sin \alpha t}{t} dt = g(0+)$$
	By Dini's Theorem\cite[Theorem 10.9]{apostol}, if the limit $g(x+)$ exists and Lebesgue integral $\int_0^\delta \frac{g(t)+g(0+)}{t} dt$ exists for some $\delta > 0$, then
	$$\lim_{\alpha to +\infty} \frac{2}{\pi} \int_0^\delta g(t) \frac{\sin \alpha t}{t} dt = g(0+)$$
	The order of Lebesgue integrals can be interchanged\cite[Theorem 10.40]{apostol},\\
	Suppose $f \in L(X)$ and $g \in L(Y)$.Then\\
	$$\int_X f(x) \left(\int_Y g(y) k(x,y) dy \right) dx = \int_Y g(y) \left( \int_X f(x) k(x,y) dx \right) dy$$
\end{synopsis}
\begin{proof}
	Consider $\int_{-\infty}^\infty f(x+t) \frac{\sin \alpha t}{\pi t} dt$. We prove that this integral is equal to the either sides.
	$$\int_{-\infty}^\infty f(x+t) \frac{\sin \alpha t}{\pi t} dt = \int_{-\infty}^{-\delta} + \int_{-\delta}^0 + \int_0^{-\delta}  + \int_{\delta}^\infty f(x+t) \frac{\sin \alpha t}{\pi t} dt $$ 
	We have, function $\frac{f(x+t)}{\pi t}$ is bounded on $(-\infty,-\delta)\cup(\delta,\infty)$, hence $\frac{f(x+t)}{\pi t}$ is Lebesgue integrable on $(-\infty,-\delta) \cup (\delta,\infty)$.\\
	
	By Riemann Lebesgue lemma, 
	$$\frac{f(x+t)}{\pi t} \in L(-\infty,-\delta) \implies \int_{-\infty}^{-\delta} f(x+t) \frac{\sin \alpha t}{\pi t} dt = 0,$$
	$$\frac{f(x+t)}{\pi t} \in L(\delta,\infty) \implies \int_{\delta}^{\infty} f(x+t) \frac{\sin \alpha t}{\pi t} dt = 0$$

	\paragraph{Case 1}
	Suppose $f$ is of bounded variation on $[x-\delta,x+\delta]$, put $g(t) = f(x+t)$ then $g$ is of bounded variation on $[-\delta,\delta]$. Thus $g$ is of bounded variation on $[0,\delta]$. Then by Jordan's Theorem
	$$\lim_{\alpha \to +\infty} \frac{2}{\pi}\int_0^\delta f(x+t)\frac{\sin \alpha t}{t} dt = \lim_{\alpha \to +\infty} \frac{2}{\pi} \int_0^\delta g(t) \frac{\sin \alpha t}{t} dt = g(0+) = f(x+)$$

	\paragraph{Case 2}
	Suppose both the limits $f(x+)$ and $f(x-)$ exists and both Lebesgue integrals
	$$ \int_0^\delta \frac{f(x+t)-f(x+)}{t} dt \text{ and } \int_0^\delta \frac{f(x-t)-f(x-)}{t} dt$$
	exists.\\

	Thus, we have $f(x+)$ exists and the Lebesgue integral $\int_0^\delta \frac{f(x+t)-f(x+)}{t} dt$ exists. Put $g(t) = f(x+t)$, then $g(0+) = f(x+)$ exists and the Lebesgue integral $\int_0^\delta \frac{g(t)-g(0+)}{t} dt$ exists, then by Dini's Theorem,
	$$\lim_{\alpha \to +\infty} \frac{2}{\pi}\int_0^\delta f(x+t)\frac{\sin \alpha t}{t} dt = \lim_{\alpha \to +\infty} \frac{2}{\pi} \int_0^\delta g(t) \frac{\sin \alpha t}{t} dt = g(0+) = f(x+)$$

	Similarly, $f(x-)$ exists and the Lebesgue integral $\int_0^\delta \frac{f(x-t)-f(x-)}{t} dt$ exists. Put $g(t) = f(x-t)$, then $g(0+) = f(x-)$ exists and the Lebesgue integral $\int_0^\delta \frac{g(t)-g(0+)}{t} dt$ exists, then by Dini's Theorem,
	\begin{align*}
		\lim_{\alpha \to +\infty} \frac{2}{\pi}\int_{-\delta}^0 f(x+t)\frac{\sin \alpha t}{t} dt
		& = \lim_{\alpha \to +\infty} \frac{2}{\pi} \int_0^\delta f(x-\tau) \frac{\sin \alpha \tau}{\tau} d\tau\\
		& = \lim_{\alpha \to +\infty} \frac{2}{\pi} \int_0^\delta g(\tau) \frac{\sin \alpha \tau}{\tau} d\tau = g(0+) = f(x-)
	\end{align*}

	Then by either cases,
	\begin{align*}
		\lim_{\alpha \to +\infty} \int_{-\infty}^\infty f(x+t) \frac{\sin \alpha t}{\pi t} dt 
		& = \lim_{\alpha \to +\infty} \int_{-\delta}^0 + \int_0^\delta f(x+t) \frac{\sin \alpha t}{\pi t} dt \\
		& = \frac{f(x+)+f(x-)}{2}
	\end{align*}

	We have, $\int_0^\alpha \cos v(u-x) dv = \frac{\sin v(u-x)}{u-x}$.
	\begin{align*}
		\lim_{\alpha \to +\infty} \int_{-\infty}^\infty f(x) \frac{ \sin \alpha t}{\pi t} dt 
		& = \lim_{\alpha \to +\infty} \int_{-\infty}^\infty f(u) \frac{ \sin \alpha (u-x)}{u-x} du,\ (\text{put }u = x+t)\\
		& = \lim_{\alpha \to +\infty} \int_{-\infty}^\infty f(u) \left( \int_0^\alpha \cos v(u-x) dv \right) du\\
		& = \lim_{\alpha \to +\infty} \int_0^\alpha \left( \int_{-\infty}^\infty f(u) \cos v(u-x) du \right) dv,\\
		& \text{since, the order of Lebesgue integrals can be reversed.}\\
		& = \int_0^\infty \left( \int_{-\infty}^\infty f(u) \cos v(u-x) du \right) dv\\
		\text{where, } \int_0^\infty \text{ is not }& \text{a Lebesgue integral, but an improper Riemann integral }
	\end{align*}
	Therefore,
	\begin{align*}
		\int_0^\infty \left( \int_{-\infty}^\infty f(u) \cos v(u-x) du \right) dv
		& = \lim_{\alpha \to +\infty} \int_{-\infty}^\infty f(x) \frac{ \sin \alpha t}{\pi t} dt \\
		& =  \frac{f(x+)+f(x-)}{2}
	\end{align*}
\end{proof}

\begin{remark}
	If a function $f$ on $(-\infty,\infty)$ is non-periodic, then it may not have a fourier series represenation. In such cases, we have fourier intergral representaion.
\end{remark}

\section{Exponential form of Fourier Integral Theorem}
	Let $f \in L(-\infty,\infty)$. Suppose $x \in \mathbb{R}$ and an interval $[x-\delta,x+\delta]$ about $x$ such that either 
	\begin{enumerate}
		\item $f$ is of bounded variation on an interval $[x-\delta,x+\delta]$ about $x$ or
		\item both limits $f(x+)$ and $f(x-)$ exists and both Lebesgue intergrals
			$$\int_0^\delta \frac{f(x+t)-f(x+)}{t} dt \text{ and }\int_0^\delta \frac{f(x-t)-f(x-)}{t} dt$$
			exists.
	\end{enumerate}
	Then, 
	$$\frac{f(x+)+f(x-)}{2} = \lim_{\alpha \to \infty} \frac{1}{2\pi} \int_{-\alpha}^\alpha \left( \int_{-\infty}^\infty f(u) e^{iv(u-x)}\ du\right) dv$$
	\begin{proof}
		Let $F(v) = \int_{-\infty}^\infty f(u) \cos v(u-x) du$. Then $F(v) = F(-v)$ and 
		\begin{align*}
			\lim_{\alpha \to \infty} \frac{1}{2\pi} \int_{-\alpha}^\alpha F(v) dv
			& = \lim_{\alpha \to \infty} \frac{1}{\pi} \int_0^\alpha \int_{-\infty}^\infty f(u) \cos v(u-x) du dv\\
			& = \frac{f(x+)+f(x-)}{2}
		\end{align*}
		Let $G(v) = \int_{-\infty}^\infty f(u) \sin v(u-x) du$. Then $G(v) = -G(-v)$ and
		$$\lim_{\alpha \to \infty} \frac{1}{2\pi} \int_{-\alpha}^\alpha G(v) dv = 0$$
		Thus 
		$$\lim_{\alpha \to \infty} \frac{1}{2\pi} \int_{-\alpha}^\alpha F(v) + iG(v) dv = \frac{f(x+)+f(x-)}{2}$$
	\end{proof}

\section{Integral Transforms}
\begin{definition}
	Integral transform $g(y)$ of $f(x)$ is a Lebesgue integral or Improper Riemann integral of the form
	$$g(y) = \int_{-\infty}^\infty K(x,y) f(x)\ dx$$, where $K$ is the kernal of the transform. We write $g = \mathscr{K}(f)$.
\end{definition}

\begin{remark}
	Integral transforms(operators) are linear operators.\\
	 ie, $\mathscr{K}(af_1 + bf_2) = a\mathscr{K}f_1 + b\mathscr{K}f_2$
\end{remark}

\begin{remark} A few commonly used integral transforms,
\begin{enumerate}
	\item Exponential Fourier Transform $\mathscr{F}$,
		$$\mathscr{F}f = \int_{-\infty}^\infty e^{-ixy}f(x)\ dx$$
	\item Fourier Cosine Transform $\mathscr{C}$,
		$$\mathscr{C}f = \int_0^\infty \cos xy f(x)\ dx$$
	\item Fourier Sine Transform $\mathscr{S}$,
		$$\mathscr{S}f = \int_0^\infty \sin xy f(x)\ dx$$
	\item Laplace Transform $\mathscr{L}$,
		$$\mathscr{L}f = \int_0^\infty e^{-xy} f(x)\ dx$$
	\item Mellin Transform $\mathscr{M}$,
		$$\mathscr{M}f = \int_0^\infty x^{y-1}f(x)\ dx$$
\end{enumerate}
\end{remark}

\begin{remark} Suppose $f(x) = 0,\ \forall x < 0$.
	$$\int_{-\infty}^\infty e^{-ixy}f(x)\ dx = \int_0^\infty e^{-ixy}f(x)\ dx = \int_0^\infty \cos xy \ f(x)\ dx + i \int_0^\infty \sin xy \ f(x)\ dx$$
	$$\mathscr{F}f = \mathscr{C}f + i\mathscr{S}f$$\\
	Therefore Fourier Cosine $\mathscr{C}$ and Sine $\mathscr{S}$ transforms are special cases of fourier integral transform, $\mathscr{F}$ provided $f$ vanishes on negative real axis.
\end{remark}

\begin{remark} Let $y = u+iv$, $f(x) = 0,\ \forall x < 0$.
	$$\int_0^\infty e^{-xy}f(x) = \int_0^\infty e^{-xu}e^{-ixv}f(x)\ dx = \int_0^\infty e^{-ixv} \phi_u(x) dx$$
	where $\phi_u(x) = e^{-xu}f(x)$.
	$$\mathscr{L}f = \mathscr{F}\phi_u$$
	Therefore Laplace transform, $\mathscr{L}$ is a special case of Fourier integral transform, $\mathscr{F}$.
\end{remark}

\begin{remark} Let $g(y) = \mathscr{F}f(x)$.
	$$g(y) = \int_{-\infty}^\infty e^{-ixy}f(x)\ dx$$
	Suppose $f$ is continuous at $x$, then by fourier integral theorem,
	\begin{align*}
		f(x)	& = \frac{1}{2\pi} \int_{-\infty}^\infty \left( \int_{-\infty}^\infty f(u) e^{iv(u-x)} du \right) dv\\
			& = \int_{-\infty}^\infty e^{-ivx} \left( \frac{1}{2\pi} \int_{-\infty}^\infty e^{ivu} f(u)\ du \right) dv\\
			& = \int_{-\infty}^\infty g(v) e^{-ivx} dv = \mathscr{F}g \text{ where } g(v) = \frac{1}{2\pi}\int_{-\infty}^\infty f(u) e^{ivu} du 
	\end{align*}
	The above function $g(v)$ gives the \textbf{inverse fourier transformation} of $f$.\\

	Let $g$ be fourier transform of $f$, then $f$ is uniquely determined by its fourier transform $g$ by,
	$$f(x) = \mathscr{F}^{-1}g(y) = \frac{1}{2\pi} \lim_{\alpha \to \infty} \int_{-\alpha}^\alpha g(y) e^{ixy} dy$$
\end{remark}

\begin{enumerate}
	\setcounter{enumi}{5}
	\item Inverse Fourier Transform $\mathscr{F}^{-1}$,
		$$\mathscr{F}^{-1}f = \int_{-\infty}^\infty \frac{e^{ixy}}{2\pi}f(x)\ dx$$
\end{enumerate}

\section{Convolutions}
\begin{definition}
	Let $f,g \in L(-\infty,\infty)$. Let $S$ be the set of all points $x$ for which the Lebesgue integral
	$$h(x) = \int_{-\infty}^\infty f(t) g(x-t) dt$$
	exists. Then the function $h : S \to \mathbb{R}$ is a convolution of $f$ and $g$. And $h = f \ast g$.
\end{definition}

\begin{remark}
	Convolution operator is commutative.\\
	ie, $ h = f \ast g = g \ast f$
\end{remark}

\begin{remark}
	Suppose $f,g$ vanishes on negative real axis, then
	$$h(x) = \int_{-\infty}^\infty f(t)\ g(x-t)\ dt = \int_{-\infty}^0 + \int_0^x  + \int_x^\infty f(t)\ g(x-t)\ dt = \int_0^x f(t)\ g(x-t)\ dt $$ 
\end{remark}

\begin{remark}
	Singularity is a point at which the convolution integral fails to exists.
\end{remark}

\begin{theorem}
	Let $f,g \in L(\mathbb{R})$ and either $f$ or $g$ is bounded in $\mathbb{R}$. Then the convoluton integral
	$$h(x) = \int_{-\infty}^\infty f(t) g(x-t) dt$$
	exists for every $x \in \mathbb{R}$ and the function $h$ so defined is bouned in $\mathbb{R}$. In addition, if the bounded function is continuous on $\mathbb{R}$, then $h$ is continuous and $h \in L(\mathbb{R})$.
\end{theorem}
\begin{synopsis}
\end{synopsis}
\begin{proof}
\end{proof}

\begin{remark}
	If $f,g$ are both unbounded, the convolution integral may not exist.
	$$\text{ eg: } f(t) = \frac{1}{\sqrt{t}},\ g(t) = \frac{1}{\sqrt{1-t}}$$
\end{remark}

\begin{theorem}
	Let $f,g \in L^2(\mathbb{R})$. Then the convolution integral $f \ast g$ exists for each $x$ in $\mathbb{R}$ and the function $h : \mathbb{R} \to \mathbb{R}$ defined by $h(x) = f \ast g (x)$ is bounded in $\mathbb{R}$.
\end{theorem}
\begin{synopsis}
\end{synopsis}
\begin{proof}
\end{proof}

\section{The Convolution Theorem for Fourier Tranforms}
\begin{theorem}
	Let $f,g \in L(\mathbb{R})$ and either $f$ or $g$ is continuous and bounded on $\mathbb{R}$. Let $h = f \ast g$. Then for every real $u$,
	$$ \int_{-\infty}^\infty h(x) e^{-ixu} dx = \left( \int_{-\infty}^\infty f(t) e^{-itu} dt \right) \left( \int_{-\infty}^\infty g(y) e^{-iyu} dy \right)$$
	The integral on the left exists both as a Lebesgue integral and an improper Riemann integral.
\end{theorem}
\begin{synopsis}
\end{synopsis}
\begin{proof}
\end{proof}

\begin{remark}[Application of Convolution Theorem]
	$$B(p,q) = \frac{\Gamma{p} \Gamma{q}}{\Gamma{p+q}},\text{ where } B(p,q) = \int_0^1 x^{p-1} (1-x)^{q-1} dx,\ \Gamma{p} = \int_0^\infty t^{p-1} e^{-t} dt$$
\end{remark}
\chapter{Multivariate Differential Calculus}
\chapter{Implicit Functions and Extremum Problems}
%\chapter{Multiple Riemann Integrals*}
%\chapter{Multiple Lebesgue Integrals*}
%\chapter{Cauchy's Theorem and the Residue Calculus*}
%\cite{rudin}

